Regex/Termination.lean
@@ -1,0 +1,37 @@
+import Regex.Basic
+
+namespace Regex
+
+variable {α : Type u} [deq : DecidableEq α] {r : Regex α} {w : List α}
+
+/-- A class of regexes that can be proven to terminate -/
+inductive classTerminates : Regex α → Prop where
+  | bot : classTerminates bot
+  | empty : classTerminates empty
+  | unit c : classTerminates (unit c)
+  | concat q r : classTerminates q → classTerminates r → classTerminates (concat q r)
+  | or q r : classTerminates q → classTerminates r → classTerminates (or q r)
+  | filterEmpty e r : classTerminates r → classTerminates (filterEmpty e r)
+  | star t r : classTerminates r → classTerminates (star t r)
+  | start : classTerminates start
+  | end' : classTerminates end'
+  | capture n r : classTerminates r → classTerminates (capture n r)
+  | backref d n : classTerminates (backref d n)
+
+/-- Rexeges constructed out of just ones in `classTerminates` terminate -/
+theorem classTerminates_terminates (r : Regex α) (hr : r.classTerminates)
+    : ∀ w s cap, r.Terminates w s cap := by
+  induction hr with
+  | bot => termination
+  | empty => termination
+  | unit c => termination
+  | concat q r _ _ qt rt => simp [concat_terminates, qt, rt]
+  | or q r _ _ qt rt => simp [or_terminates, qt, rt]
+  | filterEmpty e r _ rt => simp [filterEmpty_terminates, rt]
+  | star t r _ rt => intro r s cap; apply star_terminates_of_forall; simp [rt]
+  | start => termination
+  | end' => termination
+  | capture n r _ rt => simp [capture_terminates, rt]
+  | backref d n => termination
+
+end Regex
